basic LRU queue, maximum cache size, and eviction

disk-betree/Bounds.i.dfy
@@ -4,7 +4,7 @@ module Bounds {
   function method MaxNumChildren() : int { 32 }
   function method MaxTotalBucketWeight() : int { 8067784 }
 
-  function method MaxCacheSize() : int { 70 }
+  function method MaxCacheSize() : int { 200 }
 
   // Minimum weight a bucket needs to have before we consider flushing it.
   function method FlushTriggerWeight() : int { MaxTotalBucketWeight() / 8 }
