disk-betree/ImplFlushPolicy.i.dfy
@@ -2,6 +2,7 @@ include "ImplFlush.i.dfy"
 include "ImplGrow.i.dfy"
 include "ImplSplit.i.dfy"
 include "ImplLeaf.i.dfy"
+include "ImplEvict.i.dfy"
 include "ImplModelFlushPolicy.i.dfy"
 
 module ImplFlushPolicy {
@@ -12,6 +13,7 @@ module ImplFlushPolicy {
   import opened ImplGrow
   import opened ImplSplit
   import opened ImplLeaf
+  import opened ImplEvict
   import ImplModelFlushPolicy
   import opened ImplState
 
@@ -48,6 +50,12 @@ module ImplFlushPolicy {
     return (bestIdx, bestWeight);
   }
 
+  function method TotalCacheSize(s: ImplVariables) : (res : int)
+  requires s.Ready?
+  {
+    |s.cache| + |s.outstandingBlockReads|
+  }
+
   method getActionToSplit(k: ImplConstants, s: ImplVariables, stack: seq<BT.G.Reference>, slots: seq<uint64>, i: uint64) returns (action : ImplModelFlushPolicy.Action)
   requires 0 <= i as int < |stack|
   requires Inv(k, s)
@@ -58,13 +66,21 @@ module ImplFlushPolicy {
 
     if i == 0 {
       // Can't split root until we grow it.
-      action := ImplModelFlushPolicy.ActionGrow;
+      if TotalCacheSize(s) <= MaxCacheSize() - 1 {
+        action := ImplModelFlushPolicy.ActionGrow;
+      } else {
+        action := ImplModelFlushPolicy.ActionEvict;
+      }
     } else {
       if |s.cache[stack[i-1]].children.value| as uint64 < MaxNumChildren() as uint64 {
         if |s.cache[stack[i]].buckets| as uint64 == 1 {
           action := ImplModelFlushPolicy.ActionRepivot(stack[i]);
         } else {
-          action := ImplModelFlushPolicy.ActionSplit(stack[i-1], slots[i-1]);
+          if TotalCacheSize(s) <= MaxCacheSize() - 2 {
+            action := ImplModelFlushPolicy.ActionSplit(stack[i-1], slots[i-1]);
+          } else {
+            action := ImplModelFlushPolicy.ActionEvict;
+          }
         }
       } else {
         action := getActionToSplit(k, s, stack, slots, i-1);
@@ -72,22 +88,28 @@ module ImplFlushPolicy {
     }
   }
 
-  method getActionToFlush(k: ImplConstants, s: ImplVariables, stack: seq<BT.G.Reference>, slots: seq<uint64>) returns (action : ImplModelFlushPolicy.Action)
+  method getActionToFlush(k: ImplConstants, s: ImplVariables, stack: seq<BT.G.Reference>, slots: seq<uint64>) returns (s': ImplVariables, action : ImplModelFlushPolicy.Action)
   requires |stack| <= 40
   requires Inv(k, s)
   requires ImplModelFlushPolicy.ValidStackSlots(Ic(k), IVars(s), stack, slots)
   decreases 0x1_0000_0000_0000_0000 - |stack|
-  ensures action == ImplModelFlushPolicy.getActionToFlush(Ic(k), IVars(s), stack, slots)
+  ensures WVars(s')
+  ensures s'.Ready?
+  ensures s'.ephemeralIndirectionTable == s.ephemeralIndirectionTable
+  ensures s'.frozenIndirectionTable == s.frozenIndirectionTable
+  ensures (IVars(s'), action) == ImplModelFlushPolicy.getActionToFlush(Ic(k), old(IVars(s)), stack, slots)
   {
     ImplModelFlushPolicy.reveal_getActionToFlush();
 
     if |stack| as uint64 == 40 {
       action := ImplModelFlushPolicy.ActionFail;
+      s' := s;
     } else {
       var ref := stack[|stack| as uint64 - 1];
       var node := s.cache[ref];
       if node.children.None? || |node.buckets| == MaxNumChildren() {
         action := getActionToSplit(k, s, stack, slots, |stack| as uint64 - 1);
+        s' := s;
       } else {
         var bs := biggestSlot(node.buckets);
         var (slot, slotWeight) := bs;
@@ -97,18 +119,34 @@ module ImplFlushPolicy {
           if childref in s.cache {
             var child := s.cache[childref];
 
+            var s1 := s.(lru := LruModel.Use(s.lru, childref));
+            LruModel.LruUse(s.lru, childref);
+
             var childTotalWeight: uint64 := KMTable.computeWeightKMTSeq(child.buckets);
 
             if childTotalWeight + FlushTriggerWeight() as uint64 <= MaxTotalBucketWeight() as uint64 {
-              action := ImplModelFlushPolicy.ActionFlush(ref, slot);
+              if TotalCacheSize(s1) <= MaxCacheSize() - 1 {
+                action := ImplModelFlushPolicy.ActionFlush(ref, slot);
+                s' := s1;
+              } else {
+                action := ImplModelFlushPolicy.ActionEvict;
+                s' := s1;
+              }
             } else {
-              action := getActionToFlush(k, s, stack + [childref], slots + [slot]);
+              s', action := getActionToFlush(k, s1, stack + [childref], slots + [slot]);
             }
           } else {
-            action := ImplModelFlushPolicy.getActionToPageIn(s.cache, childref);
+            if TotalCacheSize(s) <= MaxCacheSize() - 1 {
+              action := ImplModelFlushPolicy.ActionPageIn(childref);
+              s' := s;
+            } else {
+              action := ImplModelFlushPolicy.ActionEvict;
+              s' := s;
+            }
           }
         } else {
           action := getActionToSplit(k, s, stack, slots, |stack| as uint64 - 1);
+          s' := s;
         }
       }
     }
@@ -122,38 +160,44 @@ module ImplFlushPolicy {
   requires BT.G.Root() in s.cache
   modifies io
   modifies s.ephemeralIndirectionTable.Repr
+  modifies if s.Ready? && s.frozenIndirectionTable.Some? then s.frozenIndirectionTable.value.Repr else {}
   ensures WVars(s')
-  ensures (IVars(s'), IIO(io)) == ImplModelFlushPolicy.runFlushPolicy(Ic(k), old(IVars(s)), old(IIO(io)))
+  ensures ImplModelFlushPolicy.runFlushPolicy(Ic(k), old(IVars(s)), old(IIO(io)), IVars(s'), IIO(io))
   ensures forall r | r in s.ephemeralIndirectionTable.Repr :: fresh(r) || r in old(s.ephemeralIndirectionTable.Repr)
   {
     ImplModelFlushPolicy.reveal_runFlushPolicy();
 
-    var action := getActionToFlush(k, s, [BT.G.Root()], []);
-    ImplModelFlushPolicy.getActionToFlushValidAction(Ic(k), IVars(s), [BT.G.Root()], []);
+    var s0 := s.(lru := LruModel.Use(s.lru, BT.G.Root()));
+    LruModel.LruUse(s.lru, BT.G.Root());
+    assert IM.IVars(IVars(s0)) == IM.IVars(IVars(s));
+
+    var s1, action := getActionToFlush(k, s0, [BT.G.Root()], []);
+    ImplModelFlushPolicy.getActionToFlushValidAction(Ic(k), IVars(s0), [BT.G.Root()], []);
 
     match action {
       case ActionPageIn(ref) => {
-        s' := PageInReq(k, s, io, ref);
+        s' := PageInReq(k, s1, io, ref);
       }
       case ActionSplit(parentref, slot) => {
-        s' := doSplit(k, s, parentref, s.cache[parentref].children.value[slot], slot as int);
+        s' := doSplit(k, s1, parentref, s1.cache[parentref].children.value[slot], slot as int);
       }
       case ActionRepivot(ref) => {
-        s' := repivotLeaf(k, s, ref, s.cache[ref]);
+        s' := repivotLeaf(k, s1, ref, s1.cache[ref]);
       }
       case ActionFlush(parentref, slot) => {
-        s' := flush(k, s, parentref, slot as int, 
-            s.cache[parentref].children.value[slot],
-            s.cache[s.cache[parentref].children.value[slot]]);
+        s' := flush(k, s1, parentref, slot as int, 
+            s1.cache[parentref].children.value[slot],
+            s1.cache[s1.cache[parentref].children.value[slot]]);
       }
       case ActionGrow => {
-        s' := grow(k, s);
+        s' := grow(k, s1);
       }
       case ActionEvict => {
-        s' := s;
+        s' := EvictOrDealloc(k, s1, io);
       }
       case ActionFail => {
-        s' := s;
+        print "ActionFail\n";
+        s' := s1;
       }
     }
   }
