disk-betree/ImplEvict.i.dfy
@@ -1,0 +1,113 @@
+include "ImplModelEvict.i.dfy"
+include "ImplDealloc.i.dfy"
+include "ImplSync.i.dfy"
+
+module ImplEvict {
+  import opened Impl
+  import opened ImplIO
+  import opened ImplCache
+  import opened ImplDealloc
+  import opened ImplSync
+  import ImplModelEvict
+  import opened ImplState
+
+  import opened Options
+  import opened Maps
+  import opened Sequences
+  import opened Sets
+
+  import opened NativeTypes
+
+  import LruModel
+
+  method Evict(k: ImplConstants, s: ImplVariables, ref: BT.G.Reference)
+  returns (s' : ImplVariables)
+  requires WFVars(s)
+  requires s.Ready?
+  requires ref in s.cache
+  ensures WVars(s')
+  ensures IVars(s') == ImplModelEvict.Evict(Ic(k), old(IVars(s)), ref)
+  {
+    s' := s.(cache := MapRemove1(s.cache, ref))
+     .(lru := LruModel.Remove(s.lru, ref));
+  }
+
+  method NeedToWrite(s: ImplVariables, ref: BT.G.Reference)
+  returns (b: bool)
+  requires WFVars(s)
+  requires s.Ready?
+  ensures b == ImplModelEvict.NeedToWrite(IVars(s), ref)
+  {
+    var eph := s.ephemeralIndirectionTable.Get(ref);
+    if eph.Some? && eph.value.0.None? {
+      return true;
+    }
+
+    if (s.frozenIndirectionTable.Some?) {
+      var fro := s.frozenIndirectionTable.value.Get(ref);
+      if fro.Some? && fro.value.0.None? {
+        return true;
+      }
+    }
+
+    return false;
+  }
+
+  method CanEvict(s: ImplVariables, ref: BT.G.Reference)
+  returns (b: bool)
+  requires WFVars(s)
+  requires s.Ready?
+  requires ref in s.ephemeralIndirectionTable.Contents ==>
+      s.ephemeralIndirectionTable.Contents[ref].0.Some?
+  ensures b == ImplModelEvict.CanEvict(IVars(s), ref)
+  {
+    var eph := s.ephemeralIndirectionTable.Get(ref);
+    if (eph.Some?) {
+      return BC.OutstandingWrite(ref, eph.value.0.value) !in s.outstandingBlockWrites.Values;
+    } else {
+      return true;
+    }
+  }
+
+  method EvictOrDealloc(k: ImplConstants, s: ImplVariables, io: DiskIOHandler)
+  returns (s': ImplVariables)
+  requires Inv(k, s)
+  requires s.Ready?
+  requires io.initialized()
+  requires |s.cache| > 0
+  ensures WVars(s')
+  ensures ImplModelEvict.EvictOrDealloc(Ic(k), old(IVars(s)), old(IIO(io)), IVars(s'), IIO(io))
+  ensures forall r | r in s.ephemeralIndirectionTable.Repr :: fresh(r) || r in old(s.ephemeralIndirectionTable.Repr)
+  modifies io
+  modifies s.ephemeralIndirectionTable.Repr
+  modifies if s.Ready? && s.frozenIndirectionTable.Some? then s.frozenIndirectionTable.value.Repr else {}
+  {
+    var ref := FindDeallocable(s);
+    ImplModelDealloc.FindDeallocableCorrect(IVars(s));
+
+    if ref.Some? {
+      s' := Dealloc(k, s, io, ref.value);
+    } else {
+      var ref := LruModel.Next(s.lru);
+      if ref == BT.G.Root() {
+        s' := s;
+      } else {
+        var needToWrite := NeedToWrite(s, ref);
+        if needToWrite {
+          if s.outstandingIndirectionTableWrite.None? {
+            s' := TryToWriteBlock(k, s, io, ref);
+          } else {
+            s' := s;
+          }
+        } else {
+          var canEvict := CanEvict(s, ref);
+          if canEvict {
+            s' := Evict(k, s, ref);
+          } else {
+            s' := s;
+          }
+        }
+      }
+    }
+  }
+}
