lib/LRU.i.dfy
@@ -1,0 +1,76 @@
+// A LRU-queue.
+
+include "NativeTypes.s.dfy"
+include "Sequences.s.dfy"
+
+module LruModel {
+	export S provides LruQueue, WF, I, Empty, Remove, Use, Pop, Next, LruUse, LruRemove, NativeTypes
+
+	export Internal reveals *
+	export extends S
+
+  import opened NativeTypes
+  import opened Sequences
+
+  // Index-0: Least recently used
+  // Index-1: Most recently used
+  type LruQueue = seq<uint64>
+
+  predicate {:opaque} distinct(q: seq<uint64>)
+  {
+    forall i, j | 0 <= i < |q| && 0 <= j < |q| && i != j :: q[i] != q[j]
+  }
+
+  predicate WF(q: LruQueue)
+  {
+    distinct(q)
+  }
+
+  function I(q: LruQueue) : set<uint64>
+  {
+    set i | i in q
+  }
+
+  function method Empty() : (q : LruQueue)
+  ensures I(q) == {}
+  ensures WF(q)
+  {
+    reveal_distinct();
+    []
+  }
+
+  function method Remove(q: LruQueue, i: uint64) : LruQueue
+  {
+    if |q| == 0 then [] else (
+      if Last(q) == i then Remove(DropLast(q), i) else Remove(DropLast(q), i) + [Last(q)]
+    )
+  }
+
+  function method Use(q: LruQueue, i: uint64) : LruQueue
+  {
+    Remove(q, i) + [i]
+  }
+
+  function method Next(q: LruQueue) : (i : uint64)
+  requires |I(q)| > 0
+  ensures i in I(q)
+  {
+    q[0]
+  }
+
+  function method Pop(q: LruQueue) : (LruQueue, uint64)
+  requires |I(q)| > 0
+  {
+    (q[1..], q[0])
+  }
+
+  lemma LruUse(q: LruQueue, i: uint64)
+  requires WF(q)
+  ensures WF(Use(q, i))
+  ensures I(Use(q, i)) == I(q) + {i}
+
+  lemma LruRemove(q: LruQueue, i: uint64)
+  requires WF(q)
+  ensures WF(Remove(q, i))
+  ensures I(Remove(q, i)) == I(q) - {i}
+}
